2023/P01.lean
@@ -6,47 +6,30 @@ private def loop (parse : List Char → Option ℕ) : List Char → List ℕ
                    | .none => loop parse cs'
 | [] => []
 
-def List.parse_digits := loop $
-  λ | '1' :: _ => .some 1
-    | '2' :: _ => .some 2
-    | '3' :: _ => .some 3
-    | '4' :: _ => .some 4
-    | '5' :: _ => .some 5
-    | '6' :: _ => .some 6
-    | '7' :: _ => .some 7
-    | '8' :: _ => .some 8
-    | '9' :: _ => .some 9
-    | _ => .none
+private def List.first_digit? : List Char → Option ℕ
+| c :: _ => c.as_digit?
+| _ => .none
 
-def List.parse_digits' := loop $
-  λ | '1' :: _
-    | 'o' :: 'n' :: 'e' :: _               => .some 1
-    | '2' :: _
-    | 't' :: 'w' :: 'o' :: _               => .some 2
-    | '3' :: _
-    | 't' :: 'h' :: 'r' :: 'e' :: 'e' :: _ => .some 3
-    | '4' :: _
-    | 'f' :: 'o' :: 'u' :: 'r' :: _        => .some 4
-    | '5' :: _
-    | 'f' :: 'i' :: 'v' :: 'e' :: _        => .some 5
-    | '6' :: _
-    | 's' :: 'i' :: 'x' :: _               => .some 6
-    | '7' :: _
-    | 's' :: 'e' :: 'v' :: 'e' :: 'n' :: _ => .some 7
-    | '8' :: _
-    | 'e' :: 'i' :: 'g' :: 'h' :: 't' :: _ => .some 8
-    | '9' :: _
-    | 'n' :: 'i' :: 'n' :: 'e' :: _        => .some 9
-    | _ => .none
+private def List.first_digit_name? : List Char → Option ℕ
+| 'o' :: 'n' :: 'e' :: _               => .some 1
+| 't' :: 'w' :: 'o' :: _               => .some 2
+| 't' :: 'h' :: 'r' :: 'e' :: 'e' :: _ => .some 3
+| 'f' :: 'o' :: 'u' :: 'r' :: _        => .some 4
+| 'f' :: 'i' :: 'v' :: 'e' :: _        => .some 5
+| 's' :: 'i' :: 'x' :: _               => .some 6
+| 's' :: 'e' :: 'v' :: 'e' :: 'n' :: _ => .some 7
+| 'e' :: 'i' :: 'g' :: 'h' :: 't' :: _ => .some 8
+| 'n' :: 'i' :: 'n' :: 'e' :: _        => .some 9
+| _ => .none
+
+def List.parse_q1 := loop first_digit?
+def List.parse_q2 := loop (first_digit? + first_digit_name?)
 
 def sum_by (parse_digits : List Char → List ℕ) : IO Unit := do
-  let lines ← (← IO.getStdin).lines
+  let lines ← stdin_lines
   let nums := lines.map (λ l => let ds := parse_digits l.toList
-                                let d₁ := ds.head!
-                                let d₂ := ds.reverse.head!
-                                d₁ * 10 + d₂)
-  let sum := nums.sum
+                                ds.head! * 10 + ds.last!)
   IO.println s!"values are {nums}"
-  IO.println s!"Their sum is {sum}"
+  IO.println s!"Their sum is {nums.sum}"
 
-def main : IO Unit := sum_by List.parse_digits'
+def main : IO Unit := sum_by List.parse_q2
