2023/P03.lean
@@ -31,14 +31,14 @@ def q2 : IO Unit := do
     lines.fold_sparse_grid
       (if · == '*' then .some () else .none)
       (λ idxs idx _ => idx.adjacents.foldl (λ idxs p => idxs.insert p idx) idxs)
-      .empty
+      #[|]
 
   let gear_nums : Index 2 ⊨> List ℕ :=
     lines.fold_nums
       (λ gear_nums num idxs =>
          let gears_to_add := (idxs.filterMap gear_index.find?).toSet
          gears_to_add.fold (λ gear_nums gear => gear_nums.update gear (λ _ => (num :: ·)) []) gear_nums)
-      .empty
+      #[|]
 
   let valid_gear_nums := gear_nums.filter (λ _ ns => ns.length == 2)
   let sum := valid_gear_nums.toList.sum_by (λ ⟨_, ls⟩ => ls.prod)
